propositional

Logic/Logic/System.lean
@@ -8,6 +8,10 @@ Also defines soundness and completeness.
 
 ## Main Definitions
 * `LO.System`: Proof system of logic.
+* `LO.System.Inconsistent`
+* `LO.System.Consistent`
+* `LO.System.Translation`
+* `LO.System.Compact`
 * `LO.Sound`: Soundness of the proof system.
 * `LO.Complete`: Completeness of the proof system.
 
@@ -100,8 +104,12 @@ lemma not_inconsistent_iff_consistent {𝓢 : S} :
     ¬Inconsistent 𝓢 ↔ Consistent 𝓢 :=
   ⟨fun h ↦ ⟨h⟩, by rintro ⟨h⟩; exact h⟩
 
+alias ⟨_, Consistent.not_inc⟩ := not_inconsistent_iff_consistent
+
 lemma not_consistent_iff_inconsistent {𝓢 : S} :
     ¬Consistent 𝓢 ↔ Inconsistent 𝓢 := by simp [←not_inconsistent_iff_consistent]
+
+alias ⟨_, Inconsistent.not_con⟩ := not_consistent_iff_inconsistent
 
 lemma consistent_iff_exists_unprovable {𝓢 : S} :
     Consistent 𝓢 ↔ ∃ f, 𝓢 ⊬! f := by
@@ -183,7 +191,9 @@ namespace Axiomatized
 
 variable [Axiomatized S] {𝓢 𝓢' : S}
 
-@[simp] lemma provable_axm : 𝓢 ⊢*! axm 𝓢 := fun _ hf ↦ ⟨prfAxm 𝓢 hf⟩
+@[simp] lemma provable_axm (𝓢 : S) : 𝓢 ⊢*! axm 𝓢 := fun _ hf ↦ ⟨prfAxm 𝓢 hf⟩
+
+lemma axm_subset (𝓢 : S) : axm 𝓢 ⊆ theory 𝓢 := fun p hp ↦ provable_axm 𝓢 p hp
 
 abbrev AxmSubset (𝓢 𝓢' : S) : Prop := axm 𝓢 ⊆ axm 𝓢'
 
@@ -201,6 +211,9 @@ def FiniteAxiomatizable (𝓢 : S) : Prop := ∃ 𝓕 : S, Finite 𝓕 ∧ 𝓕 
 
 lemma Consistent.of_subset {𝓢 𝓢' : S} (h𝓢 : Consistent 𝓢) (h : 𝓢' ⊆ₐₓ 𝓢) : Consistent 𝓢' :=
   h𝓢.of_le (Axiomatized.le_of_subset_axm h)
+
+lemma Inconsistent.of_supset {𝓢 𝓢' : S} (h𝓢 : Inconsistent 𝓢) (h : 𝓢 ⊆ₐₓ 𝓢') : Inconsistent 𝓢' :=
+  h𝓢.of_ge (Axiomatized.le_of_subset_axm h)
 
 namespace StrongCut
 
@@ -338,6 +351,8 @@ def DeductiveExplosion.dexp! {𝓢 : S} (h : 𝓢 ⊢! ⊥) (f : F) : 𝓢 ⊢! 
 lemma inconsistent_iff_provable_bot {𝓢 : S} :
     Inconsistent 𝓢 ↔ 𝓢 ⊢! ⊥ := ⟨fun h ↦ h ⊥, fun h f ↦ DeductiveExplosion.dexp! h f⟩
 
+alias ⟨_, inconsistent_of_provable⟩ := inconsistent_iff_provable_bot
+
 lemma consistent_iff_unprovable_bot {𝓢 : S} :
     Consistent 𝓢 ↔ 𝓢 ⊬! ⊥ := by
   simp [inconsistent_iff_provable_bot, ←not_inconsistent_iff_consistent]
@@ -383,92 +398,6 @@ lemma Deduction.inv! {p q : F} {𝓢 : S} (h : 𝓢 ⊢! p ⟶ q) : insert p �
   rcases h with ⟨b⟩; exact ⟨Deduction.inv b⟩
 
 end
-
-variable (𝓢 : S)
-
-class ModusPonens where
-  mdp {p q : F} : 𝓢 ⊢ p ⟶ q → 𝓢 ⊢ p → 𝓢 ⊢ q
-
-class Minimal extends ModusPonens 𝓢 where
-  verum              : 𝓢 ⊢ ⊤
-  imply₁ (p q : F)   : 𝓢 ⊢ p ⟶ q ⟶ p
-  imply₂ (p q r : F) : 𝓢 ⊢ (p ⟶ q ⟶ r) ⟶ (p ⟶ q) ⟶ p ⟶ r
-  conj₁  (p q : F)   : 𝓢 ⊢ p ⋏ q ⟶ p
-  conj₂  (p q : F)   : 𝓢 ⊢ p ⋏ q ⟶ q
-  conj₃  (p q : F)   : 𝓢 ⊢ p ⟶ q ⟶ p ⋏ q
-  disj₁  (p q : F)   : 𝓢 ⊢ p ⟶ p ⋎ q
-  disj₂  (p q : F)   : 𝓢 ⊢ q ⟶ p ⋎ q
-  disj₃  (p q r : F) : 𝓢 ⊢ (p ⟶ r) ⟶ (q ⟶ r) ⟶ p ⋎ q ⟶ r
-
-/-- Supplymental -/
-class EFQ where
-  efq (p : F) : 𝓢 ⊢ ⊥ ⟶ p
-
-class HasWeakLEM where
-  wlem (p : F) : 𝓢 ⊢ ~p ⋎ ~~p
-
-class HasLEM where
-  lem (p : F) : 𝓢 ⊢ p ⋎ ~p
-
-class DNE where
-  dne (p : F) : 𝓢 ⊢ ~~p ⟶ p
-
-class Dummett where
-  dummett (p q : F) : 𝓢 ⊢ (p ⟶ q) ⋎ (q ⟶ p)
-
-class Peirce where
-  peirce (p q : F) : 𝓢 ⊢ ((p ⟶ q) ⟶ p) ⟶ p
-
-/--
-  Intuitionistic Propositional Logic.
-
-  Modal companion of `𝐒𝟒`
--/
-class Intuitionistic extends Minimal 𝓢, EFQ 𝓢
-
-/--
-  Propositional Logic for Weak Law of Excluded Middle.
-
-  Modal companion of `𝐒𝟒.𝟐`
--/
-class WeakLEM extends Intuitionistic 𝓢, HasWeakLEM 𝓢
-
-/--
-  Gödel-Dummett Propositional Logic.
-
-  Modal companion of `𝐒𝟒.𝟑`
--/
-class GD extends Intuitionistic 𝓢, Dummett 𝓢
-
-/--
-  Classical Propositional Logic.
-
-  Modal companion of `𝐒𝟓`
--/
-class Classical extends Minimal 𝓢, DNE 𝓢
-
-variable {𝓢}
-
-variable [ModusPonens 𝓢]
-
-infixl:90 "⨀" => ModusPonens.mdp
-
-infixl:90 "⨀" => ModusPonens.mdp!
-
-lemma EFQ.efq! {p q} (hp : 𝓢 ⊢! p ⟶ q) (hq : 𝓢 ⊢! p) : 𝓢 ⊢! q := by
-  rcases hp with ⟨bp⟩; rcases hq with ⟨bq⟩
-  exact ⟨bp ⨀ bq⟩
-
-section EFQ
-
-variable [EFQ 𝓢]
-
-lemma efq' (b : 𝓢 ⊢ ⊥) (f : F) : 𝓢 ⊢ f := EFQ.efq f ⨀ b
-
-lemma efq'! (h : 𝓢 ⊢! ⊥) (f : F) : 𝓢 ⊢! f := by
-  rcases h with ⟨b⟩; exact ⟨efq' b f⟩
-
-end EFQ
 
 end System
 
