Logic/Propositional/Classical/Basic/Completeness.lean
@@ -8,15 +8,9 @@ namespace Propositional.Classical
 
 variable {α : Type*} {Δ : Sequent α}
 
-namespace Sequent
-
-def complexity (Δ : Sequent α) : ℕ := (Δ.map Formula.complexity).sum
-
-end Sequent
-
 namespace Derivation
 
-theorem sound : ⊢¹ Δ → Semantics.Valid Δ.disj := by
+theorem sound : ⊢¹ Δ → Semantics.Valid (Valuation α) Δ.disj := by
   intro d v
   induction d
   case axL Δ a =>
@@ -44,7 +38,7 @@ theorem sound : ⊢¹ Δ → Semantics.Valid Δ.disj := by
 
 end Derivation
 
-lemma soundness {T : Theory α} {p} : T ⊢ p → T ⊨ p := by
+lemma soundness {T : Theory (Formula α)} {p} : T ⊢! p → T ⊨[Valuation α] p := by
   rintro ⟨Γ, hΓ, d⟩ v hT
   by_contra hv
   have : ∀ v, v ⊧ p ∨ ∃ q ∈ Γ, ¬v ⊧ q := by
@@ -54,28 +48,32 @@ lemma soundness {T : Theory α} {p} : T ⊢ p → T ⊨ p := by
   have : v ⊧ q := hT.realize (hΓ q hqΓ)
   contradiction
 
-instance : Sound (Formula α) := ⟨soundness⟩
+instance (T : Theory (Formula α)) : Sound T (Semantics.models (Valuation α) T.set)  := ⟨soundness⟩
 
 section complete
 
-def consistentTheory : Set (Theory α) := { U : Theory α | System.Consistent U }
+def consistentTheory : Set (Theory (Formula α)) := { U : Theory (Formula α) | System.Consistent U }
 
-variable {T : Theory α} (consisT : Consistent T)
+variable {T : Theory (Formula α)} (consisT : Consistent T)
 open System Gentzen
 
 lemma exists_maximal_consistent_theory :
-    ∃ T', Consistent T' ∧ T ⊆ T' ∧ ∀ U, Consistent U → T' ⊆ U → U = T' :=
-  zorn_subset_nonempty { U : Theory α | Consistent U }
-    (fun c hc chain hnc ↦ ⟨⋃₀ c,
-     by simp
-        by_contra A
-        rcases compact_inconsistent A with ⟨s, hs, s_consis⟩
-        rcases Set.subset_mem_chain_of_finite c hnc chain (s := s) (Finset.finite_toSet s) hs with ⟨U, hUc, hsU⟩
-        have : Consistent (s : Set (Formula α)) := Consistent.of_subset (hc hUc) hsU
-        contradiction,
-     fun s a => Set.subset_sUnion_of_mem a⟩) T consisT
+    ∃ Z, Consistent Z ∧ T ⊆ Z ∧ ∀ U, Consistent U → Z ⊆ U → U = Z :=
+  have : ∃ Z : Set (Formula α), Consistent Z.theory ∧ T.set ⊆ Z ∧ ∀ U : Set (Formula α), Consistent U.theory → Z ⊆ U → U = Z :=
+    zorn_subset_nonempty { U : Set (Formula α) | Consistent U.theory }
+      (fun c hc chain hnc ↦ ⟨⋃₀ c,
+       by simp
+          by_contra A
+          rcases System.inconsistent_compact.mp (System.not_consistent_iff_inconsistent.mp A) with ⟨𝓕, h𝓕, fin, 𝓕_consis⟩
+          rcases Set.subset_mem_chain_of_finite c hnc chain (s := 𝓕) fin h𝓕 with ⟨U, hUc, hsU⟩
+          have : Consistent U.theory := hc hUc
+          have : ¬Consistent U.theory := (𝓕_consis.of_supset hsU).not_con
+          contradiction,
+       fun s a => Set.subset_sUnion_of_mem a⟩) T consisT
+  by rcases this with ⟨Z, con, ss, hZ⟩
+     exact ⟨Z, con, ss, by intro U conU ssU; apply Theory.setext; simpa using hZ U conU ssU⟩
 
-noncomputable def maximalConsistentTheory : Theory α :=
+noncomputable def maximalConsistentTheory : Theory (Formula α) :=
   Classical.choose (exists_maximal_consistent_theory consisT)
 
 variable {consisT}
@@ -91,8 +89,13 @@ lemma maximalConsistentTheory_maximal :
   (Classical.choose_spec (exists_maximal_consistent_theory consisT)).2.2
 
 @[simp] lemma theory_maximalConsistentTheory_eq :
+    Set.theory (theory (maximalConsistentTheory consisT)) = maximalConsistentTheory consisT :=
+  maximalConsistentTheory_maximal (U := Set.theory <| theory (maximalConsistentTheory consisT)) (by simp)
+    (by simpa [Theory.subset_def] using System.Axiomatized.axm_subset (maximalConsistentTheory consisT))
+
+@[simp] lemma theory_maximalConsistentTheory_eq' :
     theory (maximalConsistentTheory consisT) = maximalConsistentTheory consisT :=
-  maximalConsistentTheory_maximal _ (by simp) (by simp)
+  congr_arg Theory.set <| theory_maximalConsistentTheory_eq (consisT := consisT)
 
 lemma mem_or_neg_mem_maximalConsistentTheory (p) :
     p ∈ maximalConsistentTheory consisT ∨ ~p ∈ maximalConsistentTheory consisT := by
@@ -100,33 +103,33 @@ lemma mem_or_neg_mem_maximalConsistentTheory (p) :
   have hp : p ∉ maximalConsistentTheory consisT ∧ ~p ∉ maximalConsistentTheory consisT := by simpa [not_or] using A
   have : Consistent (insert p (maximalConsistentTheory consisT)) :=
     consistent_insert_iff_not_refutable.mpr
-      (unprovable_iff_not_provable.mpr <|
-        show ~p ∉ theory (maximalConsistentTheory consisT) from by simp[hp])
+      (show ~p ∉ theory (maximalConsistentTheory consisT) from by simpa using hp.2)
   have : insert p (maximalConsistentTheory consisT) ≠ maximalConsistentTheory consisT := by
-    simp[hp]
+    simp [hp, Theory.setext_iff]
   have : insert p (maximalConsistentTheory consisT) = maximalConsistentTheory consisT :=
     maximalConsistentTheory_maximal _ (by assumption) (by simp)
   contradiction
 
 lemma mem_maximalConsistentTheory_iff :
     p ∈ maximalConsistentTheory consisT ↔ maximalConsistentTheory consisT ⊢! p :=
-  ⟨fun h ↦ ⟨Deduction.axm h⟩, fun h ↦ by have : p ∈ theory (maximalConsistentTheory consisT) := h; simpa using this⟩
+  ⟨fun h ↦ ⟨System.Axiomatized.prfAxm _ h⟩, fun h ↦ by have : p ∈ theory (maximalConsistentTheory consisT) := h; simpa using this⟩
 
 lemma maximalConsistentTheory_consistent' {p} :
     p ∈ maximalConsistentTheory consisT → ~p ∉ maximalConsistentTheory consisT := by
   intro h hn
-  have : ¬Consistent (maximalConsistentTheory consisT) :=
-    inconsistent_of_provable
+  have : Inconsistent (maximalConsistentTheory consisT) :=
+    System.inconsistent_iff_provable_bot.mpr
       (by prover [mem_maximalConsistentTheory_iff.mp h, mem_maximalConsistentTheory_iff.mp hn])
+  have := this.not_con
   simp_all
 
 lemma not_mem_maximalConsistentTheory_iff :
     p ∉ maximalConsistentTheory consisT ↔ maximalConsistentTheory consisT ⊢! ~p := by
   by_cases hp : p ∈ maximalConsistentTheory consisT <;> simp[hp]
-  · apply unprovable_iff_not_provable.mpr
-    intro bnp
-    have : ¬Consistent (maximalConsistentTheory consisT) :=
-      inconsistent_of_provable (by prover [mem_maximalConsistentTheory_iff.mp hp, bnp])
+  · intro bnp
+    have : Inconsistent (maximalConsistentTheory consisT) :=
+      System.inconsistent_of_provable (by prover [mem_maximalConsistentTheory_iff.mp hp, bnp])
+    have := this.not_con
     simp_all
   · exact mem_maximalConsistentTheory_iff.mp
       (by simpa [hp] using mem_or_neg_mem_maximalConsistentTheory (consisT := consisT) p)
@@ -142,19 +145,21 @@ lemma mem_maximalConsistentTheory_or {p q} (h : p ⋎ q ∈ maximalConsistentThe
   by_contra A
   have b : maximalConsistentTheory consisT ⊢! ~p ∧ maximalConsistentTheory consisT ⊢! ~q := by
     simpa [not_or, not_mem_maximalConsistentTheory_iff] using A
-  have : ¬Consistent (maximalConsistentTheory consisT) :=
-    inconsistent_of_provable (by prover [b.1, b.2, mem_maximalConsistentTheory_iff.mp h])
+  have : Inconsistent (maximalConsistentTheory consisT) :=
+    System.inconsistent_of_provable (by prover [b.1, b.2, mem_maximalConsistentTheory_iff.mp h])
+  have := this.not_con
   simp_all
 
 lemma maximalConsistentTheory_satisfiable :
-    (Formula.atom · ∈ maximalConsistentTheory consisT) ⊧* maximalConsistentTheory consisT := ⟨by
+    (⟨(Formula.atom · ∈ maximalConsistentTheory consisT)⟩ : Valuation α) ⊧* maximalConsistentTheory consisT := ⟨by
   intro p hp
   induction p using Formula.rec' <;> simp
   case hatom => simpa
   case hnatom =>
     simpa using maximalConsistentTheory_consistent' hp
   case hfalsum =>
-    have : ¬Consistent (maximalConsistentTheory consisT) := inconsistent_of_proof (Deduction.axm hp)
+    have : Inconsistent (maximalConsistentTheory consisT) := System.inconsistent_of_provable ⟨System.Axiomatized.prfAxm _ hp⟩
+    have := this.not_con
     simp_all
   case hand p q ihp ihq =>
     exact ⟨ihp (mem_maximalConsistentTheory_and hp).1, ihq (mem_maximalConsistentTheory_and hp).2⟩
@@ -163,29 +168,29 @@ lemma maximalConsistentTheory_satisfiable :
     · left; exact ihp hp
     · right; exact ihq hq⟩
 
-lemma satisfiableTheory_of_consistent (consisT : Consistent T) : Semantics.SatisfiableSet T :=
-  ⟨(Formula.atom · ∈ maximalConsistentTheory consisT),
-    Semantics.RealizeSet.of_subset maximalConsistentTheory_satisfiable (by simp)⟩
+lemma satisfiableTheory_of_consistent (consisT : Consistent T) : Semantics.Satisfiable (Valuation α) T :=
+  ⟨⟨(Formula.atom · ∈ maximalConsistentTheory consisT)⟩,
+    Semantics.RealizeSet.of_subset maximalConsistentTheory_satisfiable (by simp [←Theory.subset_def])⟩
 
-theorem completeness! : T ⊨ p → T ⊢! p := by
-  suffices Consistent (insert (~p) T) → Semantics.SatisfiableSet (insert (~p) T) by
+theorem completeness! : T ⊨[Valuation α] p → T ⊢! p := by
+  suffices Consistent (insert (~p) T) → Semantics.Satisfiable (Valuation α) (insert (~p) T) by
     contrapose
     intro hp hs
-    have : Semantics.SatisfiableSet (insert (~p) T) :=
+    have : Semantics.Satisfiable (Valuation α) (insert (~p) T) :=
       this (consistent_insert_iff_not_refutable.mpr $ by simpa)
     rcases this with ⟨v, hv⟩
     have : v ⊧* T := Semantics.RealizeSet.of_subset hv (by simp)
-    have : v ⊧ p := hs this
+    have : v ⊧ p := hs _ this
     have : ¬v ⊧ p := by simpa using hv.realize (Set.mem_insert (~p) T)
     contradiction
   intro consis
   exact satisfiableTheory_of_consistent consis
 
-noncomputable def completeness : T ⊨ p → T ⊢ p :=
-  λ h ↦ (completeness! h).toProof
+noncomputable def completeness : T ⊨[Valuation α] p → T ⊢ p :=
+  λ h ↦ (completeness! h).prf
 
-noncomputable instance : Complete (Formula α) where
-  complete := completeness
+instance (T : Theory (Formula α)) : Complete T (Semantics.models (Valuation α) T.set)  where
+  complete := completeness!
 
 end complete
 
