Logic/AutoProver/Examples.lean
@@ -1,12 +1,12 @@
 import Logic.AutoProver.Prover
-import Logic.Propositional.Classical.Basic
-import Logic.FirstOrder.Arith.Basic
+import Logic.Propositional.Classical.Basic.Calculus
+--import Logic.FirstOrder.Arith.Basic
 
 namespace LO
 
-namespace Propositional
+namespace Propositional.Classical
 
-variable (T : Theory ℕ)
+variable (T : Theory (Formula ℕ)) {p q r : Formula ℕ}
 
 example : T ⊢! p ⋎ q ⋎ r ⋎ s ⟷ r ⋎ p ⋎ s ⋎ q ⋎ p := by tautology
 
@@ -26,8 +26,9 @@ example (h : T ⊢! p ⟷ q) : T ⊢! ~q ⟷ ~p := by prover [h]
 
 example (h : T ⊢! p ⟷ q) (hp : T ⊢! p) : T ⊢! q := by prover [h, hp]
 
-end Propositional
+end Propositional.Classical
 
+/-
 namespace FirstOrder
 open Arith
 variable (T : Theory ℒₒᵣ)
@@ -37,5 +38,6 @@ example : T ⊢! “1 < 0 → 1 < 0” := by prover
 example (h : T ⊢! “¬∀ #0 ≠ 0 → ⊥”) : T ⊢! “∀ #0 ≠ 0” := by prover [h]
 
 end FirstOrder
+-/
 
 end LO
