Logic/Logic/HilbertStyle.lean
@@ -1,0 +1,93 @@
+import Logic.Logic.System
+
+namespace LO.System
+
+variable {S F : Type*} [LogicalConnective F] [System S F]
+
+variable (𝓢 : S)
+
+class ModusPonens where
+  mdp {p q : F} : 𝓢 ⊢ p ⟶ q → 𝓢 ⊢ p → 𝓢 ⊢ q
+
+class Minimal extends ModusPonens 𝓢 where
+  verum              : 𝓢 ⊢ ⊤
+  imply₁ (p q : F)   : 𝓢 ⊢ p ⟶ q ⟶ p
+  imply₂ (p q r : F) : 𝓢 ⊢ (p ⟶ q ⟶ r) ⟶ (p ⟶ q) ⟶ p ⟶ r
+  conj₁  (p q : F)   : 𝓢 ⊢ p ⋏ q ⟶ p
+  conj₂  (p q : F)   : 𝓢 ⊢ p ⋏ q ⟶ q
+  conj₃  (p q : F)   : 𝓢 ⊢ p ⟶ q ⟶ p ⋏ q
+  disj₁  (p q : F)   : 𝓢 ⊢ p ⟶ p ⋎ q
+  disj₂  (p q : F)   : 𝓢 ⊢ q ⟶ p ⋎ q
+  disj₃  (p q r : F) : 𝓢 ⊢ (p ⟶ r) ⟶ (q ⟶ r) ⟶ p ⋎ q ⟶ r
+
+/-- Supplymental -/
+class EFQ where
+  efq (p : F) : 𝓢 ⊢ ⊥ ⟶ p
+
+class HasWeakLEM where
+  wlem (p : F) : 𝓢 ⊢ ~p ⋎ ~~p
+
+class HasLEM where
+  lem (p : F) : 𝓢 ⊢ p ⋎ ~p
+
+class DNE where
+  dne (p : F) : 𝓢 ⊢ ~~p ⟶ p
+
+class Dummett where
+  dummett (p q : F) : 𝓢 ⊢ (p ⟶ q) ⋎ (q ⟶ p)
+
+class Peirce where
+  peirce (p q : F) : 𝓢 ⊢ ((p ⟶ q) ⟶ p) ⟶ p
+
+/--
+  Intuitionistic Propositional Logic.
+
+  Modal companion of `𝐒𝟒`
+-/
+class Intuitionistic extends Minimal 𝓢, EFQ 𝓢
+
+/--
+  Propositional Logic for Weak Law of Excluded Middle.
+
+  Modal companion of `𝐒𝟒.𝟐`
+-/
+class WeakLEM extends Intuitionistic 𝓢, HasWeakLEM 𝓢
+
+/--
+  Gödel-Dummett Propositional Logic.
+
+  Modal companion of `𝐒𝟒.𝟑`
+-/
+class GD extends Intuitionistic 𝓢, Dummett 𝓢
+
+/--
+  Classical Propositional Logic.
+
+  Modal companion of `𝐒𝟓`
+-/
+class Classical extends Minimal 𝓢, DNE 𝓢
+
+variable {𝓢}
+
+variable [ModusPonens 𝓢]
+
+infixl:90 "⨀" => ModusPonens.mdp
+
+infixl:90 "⨀" => ModusPonens.mdp!
+
+lemma EFQ.efq! {p q} (hp : 𝓢 ⊢! p ⟶ q) (hq : 𝓢 ⊢! p) : 𝓢 ⊢! q := by
+  rcases hp with ⟨bp⟩; rcases hq with ⟨bq⟩
+  exact ⟨bp ⨀ bq⟩
+
+section EFQ
+
+variable [EFQ 𝓢]
+
+lemma efq' (b : 𝓢 ⊢ ⊥) (f : F) : 𝓢 ⊢ f := EFQ.efq f ⨀ b
+
+lemma efq'! (h : 𝓢 ⊢! ⊥) (f : F) : 𝓢 ⊢! f := by
+  rcases h with ⟨b⟩; exact ⟨efq' b f⟩
+
+end EFQ
+
+end LO.System
